Use constants; allow arguments

rocq-ltac2-tc-dispatch/plugin/lookup.ml
@@ -4,38 +4,86 @@ open Tac2ffi
 (* open Tac2val *)
 open Tac2externals
 
-let resolve_ltac2_safe (mp : string list) (id : string) : (unit -> unit Proofview.tactic) option =
-  let qualid = Libnames.make_qualid
-    (Names.DirPath.make (List.map Names.Id.of_string mp))
-    (Names.Id.of_string id)
+let fresh_type_scheme env (t : Tac2expr.type_scheme) : Tac2typing_env.TVar.t Tac2expr.glb_typexpr =
+  let open Tac2typing_env in
+  let (n, t) = t in
+  let subst = Array.init n (fun _ -> fresh_id env) in
+  let substf i = Tac2expr.GTypVar subst.(i) in
+  subst_type substf t
+
+let target_type : n_args:int -> int Tac2expr.glb_typexpr =
+  let open Tac2expr in
+  let unit = GTypRef (Tuple 0, []) in
+  fun ~n_args ->
+  let constr =
+    let mp = Tac2env.rocq_prefix in
+    let id = Names.Label.of_id @@ Names.Id.of_string_soft "constr" in
+    let name = Names.KerName.make mp id in
+    GTypRef (Other name, [])
   in
-  let is_unit_typ (t : int Tac2expr.glb_typexpr) : bool =
-    (* TODO: why does Init.unit have two different representations? *)
-    match t with
-    | Tac2expr.GTypRef (Tac2expr.Other ty, []) ->
-      ty = Tac2core.Core.t_unit
-    | Tac2expr.GTypRef (Tac2expr.Tuple 0, []) ->
-      true
-    | _ -> false
-  in
-  let is_unit_to_unit ((n, t) : Tac2expr.type_scheme) : bool =
-    Int.equal n 0 &&
-    match t with
-    | Tac2expr.GTypArrow (t1, t2) -> is_unit_typ t1 && is_unit_typ t2
-    | _ -> false
-  in
-  match Tac2env.locate_ltac qualid with
-  | Tac2expr.TacConstant kn ->
-    let data = Tac2env.interp_global kn in
-    if is_unit_to_unit data.Tac2env.gdata_type
-    then
-      let v = Tac2interp.eval_global kn in
-      Some (repr_to (fun1 unit unit) v)
+  let rec go n_args =
+    if n_args == 0 then
+      GTypArrow (unit, unit)
     else
-      None
-  | Tac2expr.TacAlias _ ->
-    None
-  | exception Not_found -> None
+      GTypArrow (constr, go (n_args - 1))
+  in
+  go n_args
+
+let pr_closed_type : Tac2expr.type_scheme -> Pp.t = fun t ->
+  let open Tac2typing_env in
+  let env = Tac2typing_env.empty_env ~strict:true () in
+  let (n, t) = t in
+  let subst = Array.init n (fun _ -> fresh_id env) in
+  let substf i = Tac2expr.GTypVar subst.(i) in
+  let t = subst_type substf t in
+  Tac2typing_env.pr_glbtype env t
+
+
+exception NoSuchGlobal of Names.KerName.t
+
+let resolve_ltac2_safe (r : Names.GlobRef.t) (args : Tac2val.valexpr list) : (unit -> unit Proofview.tactic) option Proofview.tactic =
+  let path =
+    let open Names.GlobRef in
+    match r with
+    | ConstRef(c) -> Some(Names.Constant.canonical c)
+    (* | IndRef(c) -> Some(Names.Ind.modpath c, Names.MutInd.user (fst c)) *)
+    | _ -> None
+  in
+  match path with
+  | None ->
+    (* Feedback.msg_debug Pp.(str "could not find constant in reference " ++ Names.GlobRef.print r); *)
+    Proofview.tclUNIT None
+  | Some path ->
+  let n_args = List.length args in
+  let check_type (ty : Tac2expr.type_scheme) : bool =
+    (* Feedback.msg_debug Pp.(str "ty: " ++ pr_closed_type ty); *)
+    let tty = target_type ~n_args in
+    (* Feedback.msg_debug Pp.(str "tty: " ++ pr_closed_type (0, tty)); *)
+    Tac2intern.check_subtype ty (0, tty)
+  in
+  try
+    let data = try Tac2env.interp_global path with | Not_found as e ->
+      let (_, info) = Exninfo.capture e in
+      Exninfo.iraise ((NoSuchGlobal path, info))
+    in
+    (* Feedback.msg_debug Pp.(str "checking types"); *)
+    if check_type data.Tac2env.gdata_type
+    then
+      let v = Tac2interp.eval_global path in
+      (* Feedback.msg_debug Pp.(str "building application"); *)
+      let v = Tac2val.apply_val v args in
+      (* Feedback.msg_debug Pp.(str "applying"); *)
+      let open Proofview.Notations in
+      v >>= fun v ->
+      (* Feedback.msg_debug Pp.(str "applied!"); *)
+      Proofview.tclUNIT (Some (repr_to (fun1 unit unit) v))
+    else
+      (* let () = Feedback.msg_debug Pp.(str "tactic type incorrect") in *)
+      Proofview.tclUNIT None
+  with
+  | NoSuchGlobal path ->
+    let () = Feedback.msg_debug Pp.(str "could not find tactic at " ++ Names.KerName.print path) in
+    Proofview.tclUNIT None
 
 
 let define s =
@@ -43,5 +91,5 @@ let define s =
 
 let () =
   define "resolve_ltac2"
-    (list string @-> string @-> ret (option (fun1 unit unit))) @@ fun modpath name ->
-    resolve_ltac2_safe modpath name
+    (reference @-> list valexpr @-> tac (option (fun1 unit unit))) @@
+    resolve_ltac2_safe
