rocq-ltac2-tc-dispatch/tests/external.v
@@ -1,13 +1,8 @@
-Require Import Stdlib.Strings.PrimString.
 Require Import Ltac2.Ltac2.
 Require Import skylabs.ltac2.tc_dispatch.lookup.
 
+Definition ext_tactic : Ltac2Ref.t. constructor. Qed.
 Ltac2 ext_tactic () := ltac1:(reflexivity).
 
-#[local] Open Scope pstring_scope.
-
 #[export]
-Instance nested_inst : Ltac2Lookup (0 = 0) := {
-  ltac2_path := "external" :: "tc_dispatch" :: "ltac2" :: "skylabs_tests" :: nil;
-  ltac2_name := "ext_tactic";
-}.
+Instance nested_inst : Dispatch (0 = 0) (CallLtac2 ext_tactic) := {}.
