rocq-ltac2-tc-dispatch/tests/nested.v
@@ -1,17 +1,14 @@
 Require Import skylabs.ltac2.tc_dispatch.lookup.
-Require Import Stdlib.Strings.PrimString.
-
-#[local] Open Scope pstring_scope.
 
 Module Import Nested.
-  Ltac2 inside_module () := ltac1:(reflexivity).
-  Instance nested_inst : Ltac2Lookup (0 = 0) := {
-    ltac2_path := "Nested" :: "nested" :: "tc_dispatch" :: "ltac2" :: "skylabs_tests" :: nil;
-    ltac2_name := "inside_module";
-  }.
+  Definition inside_module : Ltac2Ref.t. constructor. Qed.
+  Import Printf.
+  Ltac2 inside_module () :=
+    ltac1:(reflexivity).
+  Instance nested_inst : Dispatch (0 = 0) (CallLtac2 inside_module) := {}.
 End Nested.
 
 Example test_success_nested : 0 = 0.
 Proof.
-  goal_dispatch. (* Should resolve Nested.inside_module *)
+  goal_dispatch.
 Qed.
