rocq-ltac2-tc-dispatch/tests/simple.v
@@ -1,38 +1,29 @@
-Require Import Stdlib.Lists.List.
-Require Import Stdlib.Strings.PrimString.
 Require Import skylabs.ltac2.tc_dispatch.lookup.
 
-#[local] Open Scope pstring_scope.
-
 (* A simple success tactic *)
+Definition solve_true : Ltac2Ref.t. constructor. Qed.
 Ltac2 solve_true () := ltac1:(exact I).
 
 (* A tactic that prints a message *)
+Definition say_hello : Ltac2Ref.t. constructor. Qed.
 Ltac2 say_hello () := Message.print (Message.of_string "Hello from dynamic lookup!").
 
 (* Success Instance for True *)
-Instance test_true_inst : Ltac2Lookup True := {
-  ltac2_path := "simple" :: "tc_dispatch" :: "ltac2" :: "skylabs_tests" :: nil;
-  ltac2_name := "solve_true";
-}.
+Instance test_true_inst : Dispatch True (CallLtac2 solve_true) := {}.
 
 (* Success Instance for False (pointing to a printing tactic) *)
-Instance test_hello_inst : Ltac2Lookup False := {
-  ltac2_path := nil;
-  ltac2_name := "say_hello";
-}.
-
-(* A "Broken" Instance: String name does not exist *)
-Instance broken_inst : Ltac2Lookup (True -> True) := {
-  ltac2_path := nil;
-  ltac2_name := "non_existent_tactic_12345";
-}.
+Instance test_hello_inst : Dispatch False (CallLtac2 say_hello) := {}.
 
 Example test_succeed : True.
 Proof.
   goal_dispatch.
-Abort.
+Qed.
 
+Example test_succeed_print : False.
+Proof.
+  goal_dispatch.
+Fail Qed.
+Abort.
 
 (* Testing the "No Instance" failure *)
 Example test_fail_no_instance : unit.
@@ -40,8 +31,27 @@ Proof.
   Fail goal_dispatch.
 Abort.
 
-(* Testing the "Invalid Name" failure *)
-Example test_fail_bad_string : nat.
+Inductive Broken : nat -> Prop :=.
+
+Section BrokenSection.
+  Variable X : Ltac2Ref.t.
+
+  (* A "Broken" Instance: will be generalized *)
+  #[global] Instance broken_inst : Dispatch (Broken 0) (CallLtac2 X) := {}.
+End BrokenSection.
+
+(* Generalized [Lta2Ref] *)
+Example test_fail_bad_string : Broken 0.
+Proof.
+  Fail goal_dispatch. (* Triggers the None branch of our match *)
+Abort.
+
+(* Applied [Ltac2Ref]s are not supported *)
+Definition broken_ref : nat -> Ltac2Ref.t. constructor. Qed.
+Instance broken_inst_applied : Dispatch (Broken 1) (CallLtac2 (broken_ref 1)) := {}.
+
+(* Applied [Ltac2Ref] *)
+Example test_fail_bad_string : Broken 1.
 Proof.
   Fail goal_dispatch. (* Triggers the None branch of our match *)
 Abort.
