rocq-ltac2-tc-dispatch/tests/arguments.v
@@ -1,0 +1,24 @@
+Require Import skylabs.ltac2.tc_dispatch.lookup.
+
+Import Ltac2.
+Import Printf.
+
+Definition tac_with_args : nat -> bool -> Ltac2Ref.t. constructor. Qed.
+Ltac2 tac_with_args : constr -> constr -> unit -> unit :=
+  fun c1 c2 () =>
+    refine '(@eq_refl _ _ :> (Nat.eqb $c1 0  = $c2)).
+
+Instance dispatch_with_args i b : Dispatch (Nat.eqb i 0 = b) (CallLtac2 (tac_with_args i b)) := {}.
+
+Set Default Proof Mode "Classic".
+
+Goal Nat.eqb 0 0 = true.
+Proof.
+  goal_dispatch.
+Qed.
+
+Goal forall i, Nat.eqb (S i) 0 = false.
+Proof.
+  intros.
+  goal_dispatch.
+Qed.
