rocq-ltac2-tc-dispatch/tests/test_external.v
@@ -1,5 +1,5 @@
-Require Import skylabs_tests.ltac2.tc_dispatch.external.
 Require Import skylabs.ltac2.tc_dispatch.lookup.
+Require Import skylabs_tests.ltac2.tc_dispatch.external.
 
 Goal 0 = 0.
 Proof.
